State lemmas

src/Axiomatic.v
@@ -670,28 +670,38 @@ Module Valid.
   }.
   Hint Constructors pre_ex.
 
+  Definition co (ex: Execution.t) :=
+    forall eid1 eid2,
+      (exists loc
+          ex1 ord1 val1
+          ex2 ord2 val2,
+          <<LABEL: Execution.label eid1 ex = Some (Label.write ex1 ord1 loc val1)>> /\
+          <<LABEL: Execution.label eid2 ex = Some (Label.write ex2 ord2 loc val2)>>) <->
+      (eid1 = eid2 \/ ex.(Execution.co) eid1 eid2 \/ ex.(Execution.co) eid2 eid1).
+
+  Definition rf1 (ex: Execution.t) :=
+    forall eid1 ex1 ord1 loc val
+       (LABEL: Execution.label eid1 ex = Some (Label.read ex1 ord1 loc val)),
+      (<<NORF: ~ codom_rel ex.(Execution.rf) eid1>> /\ <<VAL: val = Val.default>>) \/
+      (exists eid2 ex2 ord2,
+          <<LABEL: Execution.label eid2 ex = Some (Label.write ex2 ord2 loc val)>> /\
+          <<RF: ex.(Execution.rf) eid2 eid1>>).
+
+  Definition rf2 (ex: Execution.t) :=
+    forall eid1 eid2 ex2 ord2 loc val
+       (LABEL: Execution.label eid2 ex = Some (Label.write ex2 ord2 loc val))
+       (RF: ex.(Execution.rf) eid2 eid1),
+    exists ex1 ord1,
+      <<LABEL: Execution.label eid1 ex = Some (Label.read ex1 ord1 loc val)>>.
+
+  Definition rf_wf (ex: Execution.t) := functional (ex.(Execution.rf))⁻¹.
+
   Inductive ex (p:program) (ex:Execution.t) := mk_ex {
     PRE: pre_ex p ex;
-    CO: forall eid1 eid2,
-        (exists loc
-           ex1 ord1 val1
-           ex2 ord2 val2,
-            <<LABEL: Execution.label eid1 ex = Some (Label.write ex1 ord1 loc val1)>> /\
-            <<LABEL: Execution.label eid2 ex = Some (Label.write ex2 ord2 loc val2)>>) <->
-        (eid1 = eid2 \/ ex.(Execution.co) eid1 eid2 \/ ex.(Execution.co) eid2 eid1);
-    RF1:
-      forall eid1 ex1 ord1 loc val
-        (LABEL: Execution.label eid1 ex = Some (Label.read ex1 ord1 loc val)),
-        (<<NORF: ~ codom_rel ex.(Execution.rf) eid1>> /\ <<VAL: val = Val.default>>) \/
-        (exists eid2 ex2 ord2,
-            <<LABEL: Execution.label eid2 ex = Some (Label.write ex2 ord2 loc val)>> /\
-            <<RF: ex.(Execution.rf) eid2 eid1>>);
-    RF2: forall eid1 eid2 ex2 ord2 loc val
-          (LABEL: Execution.label eid2 ex = Some (Label.write ex2 ord2 loc val))
-          (RF: ex.(Execution.rf) eid2 eid1),
-        exists ex1 ord1,
-          <<LABEL: Execution.label eid1 ex = Some (Label.read ex1 ord1 loc val)>>;
-    RF_WF: functional (ex.(Execution.rf))⁻¹;
+    CO: co ex;
+    RF1: rf1 ex;
+    RF2: rf2 ex;
+    RF_WF: rf_wf ex;
     INTERNAL: acyclic ex.(Execution.internal);
     EXTERNAL: acyclic ex.(Execution.ob);
     ATOMIC: le (ex.(Execution.rmw) ∩ (ex.(Execution.fre) ⨾ ex.(Execution.coe))) bot;
